Use pmap for programstate

theories/program/Program.v
@@ -4,6 +4,10 @@ Require Import QASMInfer.property.All.
 Require Import QASMInfer.operator.All.
 
 From Stdlib Require Import List.
+From Stdlib.FSets Require Import FMapPositive FMapFacts.
+
+Module PFacts := WFacts_fun PositiveMap.E PositiveMap.
+Module PProperties := WProperties_fun PositiveMap.E PositiveMap.
 
 Open Scope nat_scope.
 Bind Scope nat_scope with nat.
@@ -13,10 +17,12 @@ Import List.ListNotations.
 Section PROGRAM.
 
 Variable nq : nat. (* number of qubits *)
+Variable nc : nat.  (* number of classical bits *)
+
 
 (* desugared QASM instructions ================================================================== *)
 
-Inductive Instruction: Type :=
+Inductive Instruction : Type :=
 | NopInstr: Instruction
 | RotateInstr: R -> R -> R -> nat -> Instruction  (* U (theta phi lambda) qbit *)
 | CnotInstr: nat -> nat -> Instruction  (* CnotInstr a b: flip b iff a *)
@@ -30,521 +36,519 @@ Inductive Instruction: Type :=
 (* ============================================================================================== *)
 (* desugared QASM program ======================================================================= *)
 
-Record InlinedProgram: Type := {
-  IP_num_cbits: nat;
+Record InlinedProgram : Type := {
+  IP_num_cbits: nat; (* TODO: Remove? *)
   IP_instrs: Instruction;
 }.
 
 (* ============================================================================================== *)
-(* Branching for program states ================================================================= *)
+(* classical state as positive numbers ========================================================= *)
+(* `positive` is defined inductively as:
+   1. xH    (base, i.e., 1)
+   2. xI p  (append 1, i.e., multiply by 2 and add 1. notation: p~1)
+   3. xO p  (append 0, i.e., multiply by 2.           notation: p~0)
+   Note: OpenQASMCore's 0-th bit is the outermost bit in this `positive`
+   representation. Bits that is out of range are interpreted as 0s, as OpenQASM
+   initializes classical bits to 0. Doesn't care about index overflow since the
+   desugaring process ensures that won't happen. *)
 
-Record Branch: Type := {
-  B_num_clbits: nat;
-  B_qstate: Matrix nq; (* density matrix *)
-  B_cstate: total_map bool;  (* false for 0, true for 1 *)
-  B_prob: R; (* probability of the branch *)
-  B_prob_valid: (B_prob > 0)%R;
-}.
+(* No index overflow means that every classical state is uniquely represented
+   since we initialize number of bits to zero (1~0~0~...~0) and only set bits
+   within range. So we can use this to implement branch unification; two
+   branches with the same classical state, has the same positive representation
+   of classical state. *)
 
-Definition qstate_valid (b: Branch): Prop := den_valid (B_qstate b).
+Definition CState := positive.
 
-(* ============================================================================================== *)
-(* Program state ================================================================================ *)
+Fixpoint CState_init_suppl (n: nat) : positive :=
+  match n with
+  | O => xH
+  | S n' => (CState_init_suppl n')~0
+  end.
 
-Definition ProgramState: Type := list Branch.
+Definition CState_init : CState := CState_init_suppl nc.
 
-Definition ProgramState_init (num_q num_c: nat): ProgramState.
+
+Fixpoint CState_read (idx: nat) (cstate: CState) : bool :=
+  match idx, cstate with
+  | O, xO _ => false
+  | O, xI _ => true
+  | S idx', xO c | S idx', xI c => CState_read idx' c
+  | _, xH    => false  (* idx overflow -> just read 0, unreachable due to the desugaring process *)
+end.
+
+
+(* given a cstate and an index, produce two cstates by branching at the index by 0 and 1 *)
+Fixpoint CState_branch (idx: nat) (cstate: CState) : (CState * CState) :=
+  match idx, cstate with
+  (* | O, _ => (cstate, cstate)%positive *)
+  | O, xO c | O, xI c =>
+      (c~0, c~1)%positive
+  | O, xH =>
+      (1~0, 1~1)%positive (* idx overflow -> just write 0 and 1, unreachable due to the desugaring process *)
+  | S idx', xO c =>
+      let (c0, c1) := CState_branch idx' c in
+      (c0~0, c1~0)%positive
+  | S idx', xI c =>
+      let (c0, c1) := CState_branch idx' c in
+      (c0~1, c1~1)%positive
+  | S idx', xH =>
+      let (c0, c1) := CState_branch idx' xH in
+      (c0~0, c1~0)%positive  (* idx overflow -> pad with 0s, unreachable due to the desugaring process *)
+end.
+
+Lemma CState_branch_correct:
+  forall (idx: nat) (cstate: CState),
+    let (c0, c1) := CState_branch idx cstate in
+    CState_read idx c1 = true /\ CState_read idx c0 = false.
 Proof.
-  refine ([{|
-    B_num_clbits := num_c;
-    B_qstate := den_init nq;
-    B_cstate := tm_empty false;
-    B_prob := 1;
-  |}]).
-  lra.
-Defined.
-
-(* ============================================================================================== *)
-(* merging two branches ========================================================================= *)
-
-Definition Merge_branch (b0 b1: Branch): Branch.
-Proof.
-  destruct b0 eqn:ew0, b1.
-  destruct
-    (Nat.eq_dec B_num_clbits0 B_num_clbits1),
-    (tmb_equal B_cstate0 B_cstate1 B_num_clbits0) eqn:ec.
-  subst B_num_clbits1.
-  refine ({|
-    B_num_clbits := B_num_clbits0;
-    B_qstate := B_prob0 .* B_qstate0 + B_prob1 .* B_qstate1;
-    B_cstate := B_cstate0;
-    B_prob := B_prob0 + B_prob1;
-  |}).
-  lra.
-  all: exact b0.
-Defined.
-
-Definition Merge_program_state_suppl (b: Branch) (ps: ProgramState): ProgramState.
-Proof.
-  induction ps.
-  - exact [b].
-  - destruct
-    (tmb_equal (B_cstate a) (B_cstate b) (B_num_clbits a)).
-    destruct b as [nc qst cst p pv], a as [nc' qst' cst' p' pv']; simpl in *.
-    refine ({|
-      B_num_clbits := nc;
-      B_qstate := (p / (p + p'))%com .* qst + (p' / (p + p'))%com .* qst';
-      B_cstate := cst;
-      B_prob := p + p';
-    |} :: ps). (* merge *)
-      lra.
-    exact (a :: IHps). (* nop *)
-Defined.
-
-Definition Merge_program_state (ps: ProgramState): ProgramState.
-Proof.
-  destruct ps.
-  - exact [].
-  - destruct ps.
-    + exact (Merge_program_state_suppl b []).
-    + exact (Merge_program_state_suppl b (Merge_program_state_suppl b0 ps)).
-Defined.
-
-Lemma Merge_program_state_suppl_qstate_valid:
-  forall (b: Branch) (ps: ProgramState),
-  den_valid (B_qstate b) -> Forall qstate_valid ps -> Forall qstate_valid (Merge_program_state_suppl b ps).
-Proof.
-  induction ps.
-  - intros; simpl.
-    apply Forall_cons.
-    apply H.
-    apply Forall_nil.
-  - intros; simpl.
-    apply Forall_cons_iff in H0.
-    destruct H0.
-    destruct (tmb_equal (B_cstate a) (B_cstate b) (B_num_clbits a)).
-    + destruct b as [nc qst cst p pv], a as [nc' qst' cst' p' pv']; simpl in *.
-      apply Forall_cons.
-      * apply den_valid_mix.
-        all: assumption.
-      * apply H1.
-    + apply Forall_cons; auto; auto.
+  induction idx, cstate; simpl; auto.
+  all: destruct (CState_branch idx _) as [c0 c1] eqn:eb; simpl.
+  1-2: specialize (IHidx cstate).
+  3:   specialize (IHidx 1%positive).
+  all: destruct (CState_branch idx _) as [c0' c1'] eqn:eb' in IHidx.
+  all: rewrite eb in eb'.
+  all: injection eb' as Hc0 Hc1.
+  all: rewrite Hc0, Hc1.
+  all: apply IHidx.
 Qed.
 
-Lemma Merge_program_state_qstate_valid:
-  forall (branches: ProgramState),
-  Forall qstate_valid branches -> Forall qstate_valid (Merge_program_state branches).
+(* Example tests:
+Compute (CState_read 0 (1~0~1)%positive).  (* expect true *)
+Compute (CState_read 1 (1~0~1)%positive).  (* expect false *)
+Compute (CState_read 2 (1~0~1)%positive).  (* expect false (idx overflow) *)
+Compute (CState_branch 1 (CState_init_suppl 10)).  (* expect ((1~)0~0, (1~)1~0) *)
+Compute (CState_branch 3 (1~1~0)%positive).  (* expect (1~0~0~1~0, 1~1~0~1~0) *)
+*)
+
+
+(* ============================================================================================== *)
+(* Branches for different classical states ====================================================== *)
+
+Record Branch: Type := {
+  B_qstate: Matrix nq; (* density matrix *)
+  B_prob: R; (* probability of the branch *)
+  (* B_prob_valid: (B_prob > 0)%R; TODO: prove later that prob is always > 0 separately (for equivalence) *)
+}.
+
+Definition Branch_valid (b: Branch): Prop := den_valid (B_qstate b) /\ (B_prob b > 0)%R.
+
+Definition Branch_init: Branch := {|
+    B_qstate := den_init nq;
+    B_prob := 1;
+  |}.
+
+Definition Branch_merge (b0 b1: Branch): Branch :=
+  {|
+    B_qstate :=
+      (B_prob b0 / (B_prob b0 + B_prob b1))%com .* B_qstate b0 +
+      (B_prob b1 / (B_prob b0 + B_prob b1))%com .* B_qstate b1;
+    B_prob := B_prob b0 + B_prob b1;
+  |}.
+
+Lemma Branch_merge_valid: forall (b0 b1: Branch),
+  Branch_valid b0 -> Branch_valid b1 -> Branch_valid (Branch_merge b0 b1).
 Proof.
-  intros; simpl.
-  induction branches as [|b0[|b1 t] ].
-  - apply Forall_nil.
-  - apply H.
-  - apply Forall_cons_iff in H; destruct H.
-    apply Forall_cons_iff in H0; destruct H0.
-    apply Merge_program_state_suppl_qstate_valid.
-    all: auto.
-    apply Merge_program_state_suppl_qstate_valid.
-    all: auto.
+  intros b0 b1 [Hvalid0 Hprob0] [Hvalid1 Hprob1].
+  unfold Branch_merge, Branch_valid in *; simpl.
+  split.
+  apply den_valid_mix.
+  all: try lra; assumption.
+Qed.
+
+
+(* ============================================================================================== *)
+(* Program state as pos -> branch, i.e., map from cstate to qstate and probability ============== *)
+(* This is possible thanks to branch unification ================================================ *)
+
+Definition ProgramState: Type := PositiveMap.t Branch.
+
+(* every qstate in ProgramState is valid *)
+Definition ProgramState_valid (ps: ProgramState): Prop :=
+  forall (cstate: positive) (branch: Branch),
+    PositiveMap.MapsTo cstate branch ps -> Branch_valid branch.
+
+Definition ProgramState_init: ProgramState :=
+  PositiveMap.add CState_init Branch_init (PositiveMap.empty Branch).
+
+Definition ProgramState_merge (ps0 ps1: ProgramState): ProgramState :=
+  PositiveMap.fold (fun cstate branch acc =>
+    match PositiveMap.find cstate acc with
+    | Some branch' =>
+        PositiveMap.add cstate (Branch_merge branch branch') acc
+    | None =>
+        PositiveMap.add cstate branch acc
+    end) ps0 ps1.
+
+Lemma ProgramState_map_valid: forall (f: Branch -> Branch) (ps: ProgramState),
+  ProgramState_valid ps -> (forall b, Branch_valid b -> Branch_valid (f b)) ->
+  ProgramState_valid (PositiveMap.map f ps).
+Proof.
+  unfold ProgramState_valid.
+  intros f ps Hps Hf_valid cstate branch' Hmaps.
+  apply PFacts.map_mapsto_iff in Hmaps.
+  destruct Hmaps as [branch [Hb' Hfind]].
+  specialize (Hps cstate branch).
+  rewrite Hb'.
+  apply Hf_valid.
+  apply Hps.
+  apply Hfind.
+Qed.
+
+Lemma ProgramState_merge_valid: forall (ps0 ps1: ProgramState),
+  ProgramState_valid ps0 -> ProgramState_valid ps1 ->
+  ProgramState_valid (ProgramState_merge ps0 ps1).
+Proof.
+  intros ps0 ps1 Hps0 Hps1.
+  unfold ProgramState_merge.
+  apply PProperties.fold_rec_nodep.
+  assumption.
+  intros cstate_fold branch_fold acc Hmaps_fold Hacc_valid.
+  destruct (PositiveMap.find cstate_fold acc) eqn:Hfind.
+  - apply PFacts.find_mapsto_iff in Hfind.
+    intros cstate' branch' Hmaps'.
+    apply PFacts.add_mapsto_iff in Hmaps'.
+    destruct Hmaps' as [[Hcstate_eq Hbranch_eq] | [Hcstate_neq Hmaps_acc]].
+    + rewrite <- Hbranch_eq.
+      unfold ProgramState_valid in *.
+      apply Branch_merge_valid.
+      * apply (Hps0 cstate_fold branch_fold Hmaps_fold).
+      * apply (Hacc_valid cstate').
+        rewrite <- Hcstate_eq.
+        assumption.
+    + apply (Hacc_valid cstate' branch' Hmaps_acc).
+  - apply PFacts.not_find_in_iff in Hfind.
+    intros cstate' branch' Hmaps'.
+    apply PFacts.add_mapsto_iff in Hmaps'.
+    destruct Hmaps' as [[Hcstate_eq Hbranch_eq] | [Hcstate_neq Hmaps_acc]].
+    + rewrite <- Hbranch_eq.
+      unfold ProgramState_valid in *.
+      apply (Hps0 cstate_fold branch_fold Hmaps_fold).
+    + apply (Hacc_valid cstate' branch' Hmaps_acc).
 Qed.
 
 (* ============================================================================================== *)
 (* execution ==================================================================================== *)
 
-Fixpoint Execute_rotate_instr (theta phi lambda: R) (target: nat) (branches: ProgramState): ProgramState.
-Proof.
-  destruct branches as [|[nc qstate cstate prob Hp] t].
-  - exact [].
-  - destruct (lt_dec target nq).
-    + exact ({|
-        B_num_clbits := nc;
-        B_qstate := den_uop (mat_single nq target (mat_rot theta phi lambda)) qstate ;
-        B_cstate := cstate;
-        B_prob := prob;
-        B_prob_valid := Hp;
-      |} :: (Execute_rotate_instr theta phi lambda target t)).
-    + exact ({|
-        B_num_clbits := nc;
-        B_qstate := qstate;
-        B_cstate := cstate;
-        B_prob := prob;
-        B_prob_valid := Hp;
-      |} :: (Execute_rotate_instr theta phi lambda target t)).  (* nop *)
-Defined.
+Definition Execute_rotate_instr_branch (theta phi lambda: R) (target: nat) (branch: Branch): Branch :=
+  {|
+    B_qstate := den_uop (mat_single nq target (mat_rot theta phi lambda)) (B_qstate branch) ;
+    B_prob := B_prob branch;
+  |}.
 
-Fixpoint Execute_cnot_instr (control target: nat) (branches: ProgramState): ProgramState.
-Proof.
-  destruct branches as [|[nc qstate cstate prob Hp] t].
-  - exact [].
-  - destruct (ge_dec nq 2), (lt_dec control nq), (lt_dec target nq).
-    exact ({|
-      B_num_clbits := nc;
-      B_qstate := den_uop (mat_cnot control target) qstate;
-      B_cstate := cstate;
-      B_prob := prob;
-      B_prob_valid := Hp;
-      |} :: (Execute_cnot_instr control target t)).
-    all: refine ({|
-      B_num_clbits := nc;
-      B_qstate := qstate;
-      B_cstate := cstate;
-      B_prob := prob;
-      B_prob_valid := Hp;
-    |} :: (Execute_cnot_instr control target t)).  (* nop *)
-Defined.
+Definition Execute_rotate_instr (theta phi lambda: R) (target: nat) (ps: ProgramState): ProgramState :=
+  PositiveMap.map (Execute_rotate_instr_branch theta phi lambda target) ps.
 
-Fixpoint Execute_swap_instr (q1 q2: nat) (branches: ProgramState): ProgramState.
-Proof.
-  destruct branches as [|[nc qstate cstate prob Hp] t].
-  - exact [].
-  - destruct (lt_dec q1 nq), (lt_dec q2 nq).
-    exact ({|
-      B_num_clbits := nc;
-      B_qstate := den_uop (mat_swap q1 q2) qstate;
-      B_cstate := cstate;
-      B_prob := prob;
-      B_prob_valid := Hp;
-      |} :: (Execute_swap_instr q1 q2 t)).
-    all: exact ({|
-        B_num_clbits := nc;
-        B_qstate := qstate;
-        B_cstate := cstate;
-        B_prob := prob;
-        B_prob_valid := Hp;
-      |} :: (Execute_swap_instr q1 q2 t)).  (* nop *)
-Defined.
 
-Fixpoint Execute_measure_instr (qbit cbit: nat) (branches: ProgramState): ProgramState.
-Proof.
-  destruct branches as [|[nc qstate cstate prob Hp] t].
-  - exact [].
-  - destruct (lt_dec qbit nq).
-    + specialize (com_real (den_prob_0 qbit qstate)) as prob0.
-      specialize (com_real (den_prob_1 qbit qstate)) as prob1.
-      destruct (Rgt_dec prob0 0), (Rgt_dec prob1 0).
-      * refine ({|
-          B_num_clbits := nc;
-          B_qstate := den_measure_0 qbit qstate;
-          B_cstate := tm_update cstate cbit false;
-          B_prob := prob * prob0;
-        |} :: {|
-          B_num_clbits := nc;
-          B_qstate := den_measure_1 qbit qstate;
-          B_cstate := tm_update cstate cbit true;
-          B_prob := prob * prob1;
-        |} ::
-        (Execute_measure_instr qbit cbit t)).
-        all: try nra.
-      * refine ({|
-          B_num_clbits := nc;
-          B_qstate := den_measure_0 qbit qstate;
-          B_cstate := tm_update cstate cbit false;
-          B_prob := prob * prob0;
-        |} ::
-        (Execute_measure_instr qbit cbit t)).
-        nra.
-      * refine ({|
-          B_num_clbits := nc;
-          B_qstate := den_measure_1 qbit qstate;
-          B_cstate := tm_update cstate cbit true;
-          B_prob := prob * prob1;
-        |} ::
-        (Execute_measure_instr qbit cbit t)).
-        nra.
-      * exact (Execute_measure_instr qbit cbit t).  (* nop *)
-  + exact (Execute_measure_instr qbit cbit t).  (* nop *)
-Defined.
+Definition Execute_cnot_instr_branch (control target: nat) (branch: Branch): Branch :=
+  {|
+    B_qstate := den_uop (mat_cnot control target) (B_qstate branch) ;
+    B_prob := B_prob branch;
+  |}.
 
-Fixpoint Execute_reset_instr (target: nat) (branches: ProgramState): ProgramState.
-Proof.
-  destruct branches as [|[nc qstate cstate prob Hp] t].
-  - exact [].
-  - destruct (lt_dec target nq).
-    + exact ({|
-        B_num_clbits := nc;
-        B_qstate := den_reset target qstate;
-        B_cstate := cstate;
-        B_prob := prob;
-        B_prob_valid := Hp;
-      |} :: (Execute_reset_instr target t)).
-    + exact ({|
-        B_num_clbits := nc;
-        B_qstate := qstate;
-        B_cstate := cstate;
-        B_prob := prob;
-        B_prob_valid := Hp;
-      |} :: (Execute_reset_instr target t)).  (* nop *)
-Defined.
+Definition Execute_cnot_instr (control target: nat) (ps: ProgramState): ProgramState :=
+  PositiveMap.map (Execute_cnot_instr_branch control target) ps.
 
-Fixpoint Execute_suppl_old (ir: nat) (instr: Instruction) (branches: ProgramState): ProgramState :=
-  match ir with
-  | O => branches
-  | S ir' => (
-    match instr with
-    | NopInstr                            => branches
-    | RotateInstr theta phi lambda target => Execute_rotate_instr theta phi lambda target branches
-    | CnotInstr control target            => Execute_cnot_instr control target branches
-    | SwapInstr q1 q2                     => Execute_swap_instr q1 q2 branches
-    | MeasureInstr qbit cbit              => Merge_program_state (Execute_measure_instr qbit cbit branches)
-    | SeqInstr i1 i2                      => Execute_suppl_old ir' i2 (Execute_suppl_old ir' i1 branches)
-    | IfInstr cbit cond subinstr          => (
-        concat (map (fun b =>
-          if (eqb (B_cstate b cbit) cond)
-          then Execute_suppl_old ir' subinstr [b]
-          else [b]) branches)
-    )
-    | ResetInstr target                   => Execute_reset_instr target branches
-    end
-  )
+
+Definition Execute_swap_instr_branch (q1 q2: nat) (branch: Branch): Branch :=
+  {|
+    B_qstate := den_uop (mat_swap q1 q2) (B_qstate branch) ;
+    B_prob := B_prob branch;
+  |}.
+
+Definition Execute_swap_instr (q1 q2: nat) (ps: ProgramState): ProgramState :=
+  PositiveMap.map (Execute_swap_instr_branch q1 q2) ps.
+
+
+Definition Execute_measure_instr_branch (qbit cbit: nat) (cstate: CState) (branch: Branch): ProgramState :=
+  let prob0 := com_real (den_prob_0 qbit (B_qstate branch)) in
+  let prob1 := com_real (den_prob_1 qbit (B_qstate branch)) in
+  let (cstate0, cstate1) := CState_branch cbit cstate in
+  match (Rgt_dec prob0 0), (Rgt_dec prob1 0) with
+  | left _, left _ => (* true, true *)
+      PositiveMap.add cstate0 {|
+          B_qstate := den_measure_0 qbit (B_qstate branch);
+          B_prob := B_prob branch * prob0;
+        |}
+        (PositiveMap.add cstate1 {|
+          B_qstate := den_measure_1 qbit (B_qstate branch);
+          B_prob := B_prob branch * prob1;
+        |} (PositiveMap.empty Branch))
+  | left _, right _ => (* true, false *)
+      PositiveMap.add cstate0 {|
+          B_qstate := den_measure_0 qbit (B_qstate branch);
+          B_prob := B_prob branch * prob0;
+        |} (PositiveMap.empty Branch)
+  | right _, left _ => (* false, true *)
+      PositiveMap.add cstate1 {|
+          B_qstate := den_measure_1 qbit (B_qstate branch);
+          B_prob := B_prob branch * prob1;
+        |} (PositiveMap.empty Branch)
+  | right _, right _ => (* false, false *)
+      PositiveMap.empty Branch
   end.
 
-Fixpoint Execute_suppl (instr: Instruction) (branches: ProgramState): ProgramState :=
+Definition Execute_measure_instr (qbit cbit: nat) (ps: ProgramState): ProgramState :=
+  PositiveMap.fold (fun cstate branch acc =>
+    ProgramState_merge acc (Execute_measure_instr_branch qbit cbit cstate branch)
+  ) ps (PositiveMap.empty Branch).
+
+
+Definition Execute_reset_instr_branch (target: nat) (branch: Branch): Branch :=
+  {|
+    B_qstate := den_reset target (B_qstate branch);
+    B_prob := B_prob branch;
+  |}.
+
+Definition Execute_reset_instr (target: nat) (ps: ProgramState): ProgramState :=
+  PositiveMap.map (Execute_reset_instr_branch target) ps.
+
+
+Fixpoint Execute_suppl (instr: Instruction) (ps: ProgramState): ProgramState :=
     match instr with
-    | NopInstr                            => branches
-    | RotateInstr theta phi lambda target => Execute_rotate_instr theta phi lambda target branches
-    | CnotInstr control target            => Execute_cnot_instr control target branches
-    | SwapInstr q1 q2                     => Execute_swap_instr q1 q2 branches
-    | MeasureInstr qbit cbit              => Merge_program_state (Execute_measure_instr qbit cbit branches)
-    | SeqInstr i1 i2                      => Execute_suppl i2 (Execute_suppl i1 branches)
-    | IfInstr cbit cond subinstr          => (
-        concat (map (fun b =>
-          if (eqb (B_cstate b cbit) cond)
-          then Execute_suppl subinstr [b]
-          else [b]) branches)
-    )
-    | ResetInstr target                   => Execute_reset_instr target branches
+    | NopInstr                            => ps
+    | RotateInstr theta phi lambda target => Execute_rotate_instr theta phi lambda target ps
+    | CnotInstr control target            => Execute_cnot_instr control target ps
+    | SwapInstr q1 q2                     => Execute_swap_instr q1 q2 ps
+    | MeasureInstr qbit cbit              => Execute_measure_instr qbit cbit ps
+    | SeqInstr i1 i2                      => Execute_suppl i2 (Execute_suppl i1 ps)
+    | IfInstr cbit cond subinstr          => PositiveMap.fold (fun cstate b acc =>
+        let ps_single := PositiveMap.add cstate b (PositiveMap.empty Branch) in
+        if (eqb (CState_read cbit cstate) cond)
+        then Execute_suppl subinstr ps_single
+        else ps_single) ps (PositiveMap.empty Branch)
+    | ResetInstr target                   => Execute_reset_instr target ps
     end.
 
 Definition Execute (program: InlinedProgram): ProgramState :=
-  Execute_suppl
-    (IP_instrs program)
-    (ProgramState_init nq (IP_num_cbits program)).
+  Execute_suppl (IP_instrs program) ProgramState_init.
 
-Fixpoint Cstate_to_binary_little_endian (n: nat) (cstate: total_map bool) (acc: nat): nat := match n with
+Fixpoint Cstate_to_binary_little_endian (n: nat) (cstate: CState) (acc: nat): nat := match n with
   | O => acc
-  | S n' => let bit := if (cstate n') then 1 else 0 in
+  | S n' => let bit := if (CState_read n' cstate) then 1 else 0 in
             Cstate_to_binary_little_endian n' cstate (2 * acc + bit)
 end.
 
-Definition Cstate_to_binary (num_cbits: nat) (cstate: total_map bool) := Cstate_to_binary_little_endian num_cbits cstate O.
+Definition Cstate_to_binary (num_cbits: nat) (cstate: CState) := Cstate_to_binary_little_endian num_cbits cstate O.
 
 (*  0 -> true
     1 -> false     ===> 1011 (value of 0 is the leftmost bit in the result) (big endian)
     2 -> true      ===> In qasm, they use little endian so have to reverse it
     3 -> true *)
 
+Definition Calculate_prob (ps: ProgramState): PositiveMap.t R :=
+  PositiveMap.map (fun b => B_prob b) ps.
 
-Fixpoint Calculate_prob (num_cbits: nat) (branches: ProgramState): total_map R :=
-  match branches with
-  | [] => tm_empty R0
-  | b :: t =>
-    let prev := Calculate_prob num_cbits t in
-    let key := Cstate_to_binary num_cbits (B_cstate b) in
-    tm_update prev key (prev key + B_prob b)%R
-  end.
-
-Definition Execute_and_calculate_prob (program: InlinedProgram): total_map R :=
-  Calculate_prob (IP_num_cbits program) (Execute program).
+Definition Execute_and_calculate_prob (program: InlinedProgram): PositiveMap.t R :=
+  Calculate_prob (Execute program).
 
 (* ============================================================================================== *)
 (* Proof about quantum states =================================================================== *)
 
-Lemma Execute_rotate_instr_quantum_state_density:
-  forall (theta phi lambda: R) (target: nat) (branches: ProgramState),
-  Forall qstate_valid branches ->
-  Forall qstate_valid (Execute_rotate_instr theta phi lambda target branches).
+Lemma Execute_rotate_instr_valid:
+  forall (theta phi lambda: R) (target: nat) (ps: ProgramState),
+  ProgramState_valid ps ->
+  ProgramState_valid (Execute_rotate_instr theta phi lambda target ps).
 Proof.
   intros.
-  induction branches.
-  - apply H.
-  - destruct a.
-    apply Forall_cons_iff in H.
-    destruct H as [H Ht].
-    simpl in *.
-    destruct (lt_dec target nq).
-    + apply Forall_cons; simpl.
-      apply den_valid_uop.
-      apply mat_single_unitary.
-      apply mat_rot_unitary.
-      assumption.
-      apply IHbranches.
-      apply Ht.
-    + apply Forall_cons; simpl.
-      apply H.
-      apply IHbranches.
-      apply Ht.
+  apply (ProgramState_map_valid _ _ H).
+  intros b [Hvalid Hprob].
+  unfold Execute_rotate_instr_branch, Branch_valid in *; simpl.
+  split.
+  apply den_valid_uop.
+  apply mat_single_unitary.
+  apply mat_rot_unitary.
+  assumption.
+  assumption.
 Qed.
 
-Lemma Execute_cnot_instr_quantum_state_density:
-  forall (control target: nat) (branches: ProgramState),
-  Forall qstate_valid branches -> Forall qstate_valid (Execute_cnot_instr control target branches).
+Lemma Execute_cnot_instr_valid:
+  forall (control target: nat) (ps: ProgramState),
+  ProgramState_valid ps ->
+  ProgramState_valid (Execute_cnot_instr control target ps).
 Proof.
   intros.
-  induction branches.
-  - apply H.
-  - destruct a.
-    apply Forall_cons_iff in H.
-    destruct H as [H Ht].
-    simpl in *.
-    destruct (ge_dec nq 2), (lt_dec control nq), (lt_dec target nq).
-    { apply Forall_cons.
-      simpl.
-      apply den_valid_uop.
-      apply mat_cnot_unitary.
-      assumption.
-      apply IHbranches.
-      apply Ht. }
-      all: apply Forall_cons.
-      all: simpl; try apply H.
-      all: apply IHbranches.
-      all: apply Ht.
+  apply (ProgramState_map_valid _ _ H).
+  intros b [Hvalid Hprob].
+  unfold Execute_rotate_instr_branch, Branch_valid in *; simpl.
+  split.
+  apply den_valid_uop.
+  apply mat_cnot_unitary.
+  assumption.
+  assumption.
 Qed.
 
-Lemma Execute_swap_instr_quantum_state_density:
-  forall (q1 q2: nat) (branches: ProgramState),
-  Forall qstate_valid branches -> Forall qstate_valid (Execute_swap_instr q1 q2 branches).
+Lemma Execute_swap_instr_valid:
+  forall (q1 q2: nat) (ps: ProgramState),
+  ProgramState_valid ps -> ProgramState_valid (Execute_swap_instr q1 q2 ps).
 Proof.
   intros.
-  induction branches.
-  - apply H.
-  - destruct a.
-    apply Forall_cons_iff in H.
-    destruct H as [H Ht].
-    simpl in *.
-    destruct (lt_dec q1 nq), (lt_dec q2 nq).
-    { apply Forall_cons.
-      simpl.
-      apply den_valid_uop.
-      apply mat_swap_unitary.
-      assumption.
-      apply IHbranches.
-      apply Ht. }
-      all: apply Forall_cons.
-      all: simpl; try apply H.
-      all: apply IHbranches.
-      all: apply Ht.
+  apply (ProgramState_map_valid _ _ H).
+  intros b [Hvalid Hprob].
+  unfold Execute_rotate_instr_branch, Branch_valid in *; simpl.
+  split.
+  apply den_valid_uop.
+  apply mat_swap_unitary.
+  assumption.
+  assumption.
 Qed.
 
-Lemma Execute_measure_instr_quantum_state_density:
-  forall (qbit cbit: nat) (branches: ProgramState),
-  Forall qstate_valid branches -> Forall qstate_valid (Execute_measure_instr qbit cbit branches).
+
+Lemma Execute_measure_instr_branch_valid:
+  forall (qbit cbit: nat) (cstate: CState) (branch: Branch),
+  Branch_valid branch ->
+  ProgramState_valid (Execute_measure_instr_branch qbit cbit cstate branch).
+Proof.
+  intros qbit cbit cstate branch [Hvalid Hprob].
+  unfold Execute_measure_instr_branch, ProgramState_valid.
+  intros cstate' branch'.
+  destruct (CState_branch cbit cstate) as [cstate0 cstate1].
+  destruct (Rgt_dec (com_real (den_prob_0 qbit (B_qstate branch))) 0) eqn:Hdec0,
+           (Rgt_dec (com_real (den_prob_1 qbit (B_qstate branch))) 0) eqn:Hdec1;
+           unfold den_prob_0, den_prob_1, com_real in *.
+  - intros Hmaps.
+    apply PFacts.add_mapsto_iff in Hmaps.
+    destruct Hmaps as [[Hcstate_eq Hbranch_eq] | [Hcstate_neq Hmaps]].
+    + rewrite <- Hbranch_eq.
+      unfold Branch_valid; simpl.
+      split.
+      * apply den_valid_measure.
+        apply mat_proj0_projection.
+        apply Hvalid.
+        apply com_proj_neq_fst.
+        simpl; lra.
+      * nra.
+    + apply PFacts.add_mapsto_iff in Hmaps.
+      destruct Hmaps as [[Hcstate_eq Hbranch_eq] | [Hcstate_neq' Hmaps]].
+      * rewrite <- Hbranch_eq.
+        unfold Branch_valid; simpl.
+        split.
+        -- apply den_valid_measure.
+          apply mat_proj1_projection.
+          apply Hvalid.
+          apply com_proj_neq_fst.
+          simpl; lra.
+        -- nra.
+      * apply PFacts.empty_mapsto_iff in Hmaps.
+        contradiction.
+  - intros Hmaps.
+    apply PFacts.add_mapsto_iff in Hmaps.
+    destruct Hmaps as [[Hcstate_eq Hbranch_eq] | [Hcstate_neq Hmaps]].
+    + rewrite <- Hbranch_eq.
+      unfold Branch_valid; simpl.
+      split.
+      * apply den_valid_measure.
+        apply mat_proj0_projection.
+        apply Hvalid.
+        apply com_proj_neq_fst.
+        simpl; lra.
+      * nra.
+    + apply PFacts.empty_mapsto_iff in Hmaps.
+      contradiction.
+  - intros Hmaps.
+    apply PFacts.add_mapsto_iff in Hmaps.
+    destruct Hmaps as [[Hcstate_eq Hbranch_eq] | [Hcstate_neq Hmaps]].
+    + rewrite <- Hbranch_eq.
+      unfold Branch_valid; simpl.
+      split.
+      * apply den_valid_measure.
+        apply mat_proj1_projection.
+        apply Hvalid.
+        apply com_proj_neq_fst.
+        simpl; lra.
+      * nra.
+    + apply PFacts.empty_mapsto_iff in Hmaps.
+      contradiction.
+  - intros Hmaps.
+    apply PFacts.empty_mapsto_iff in Hmaps.
+    contradiction.
+Qed.
+
+Lemma Execute_measure_instr_valid:
+  forall (qbit cbit: nat) (ps: ProgramState),
+  ProgramState_valid ps -> ProgramState_valid (Execute_measure_instr qbit cbit ps).
+Proof.
+  intros qbit cbit ps Hpsvalid.
+  unfold Execute_measure_instr.
+  apply PProperties.fold_rec_nodep.
+  - unfold ProgramState_valid; intros.
+    apply PFacts.empty_mapsto_iff in H.
+    contradiction.
+  - intros cstate_fold branch_fold acc Hmaps_fold Hacc_valid.
+    apply (ProgramState_merge_valid _ _ Hacc_valid).
+    apply Execute_measure_instr_branch_valid.
+    apply (Hpsvalid cstate_fold branch_fold Hmaps_fold).
+Qed.
+
+
+Lemma Execute_reset_instr_valid:
+  forall (target: nat) (ps: ProgramState),
+  ProgramState_valid ps -> ProgramState_valid (Execute_reset_instr target ps).
 Proof.
   intros.
-  induction branches.
-  - apply H.
-  - destruct a.
-    apply Forall_cons_iff in H.
-    destruct H as [H Ht].
-    simpl in *.
-    destruct (lt_dec qbit nq).
-    + destruct
-      (Rgt_dec (com_real (den_prob_0 qbit B_qstate0)) 0),
-      (Rgt_dec (com_real (den_prob_1 qbit B_qstate0)) 0).
-      all: try repeat apply Forall_cons; simpl.
-      all: unfold den_measure_0, den_measure_1 in *.
-      all: try apply den_valid_measure.
-      all: unfold den_prob_0, den_prob_1, den_prob in *.
-      all: try apply H.
-      all: try apply mat_proj0_projection; try apply mat_proj1_projection.
-      all: unfold com_real in *.
-      all: try apply com_proj_neq_fst.
-      all: unfold NTC, INR; simpl; try lra.
-      all: apply IHbranches.
-      all: apply Ht.
-    + apply IHbranches.
-      apply Ht.
+  apply (ProgramState_map_valid _ _ H).
+  intros b [Hvalid Hprob].
+  unfold Execute_reset_instr_branch, Branch_valid in *; simpl.
+  split.
+  apply den_valid_reset.
+  apply Hvalid.
+  assumption.
 Qed.
 
-Lemma Execute_reset_instr_quantum_state_density:
-  forall (target: nat) (branches: ProgramState),
-  Forall qstate_valid branches -> Forall qstate_valid (Execute_reset_instr target branches).
-Proof.
-  intros.
-  induction branches.
-  - simpl.
-    apply H.
-  - destruct a.
-    apply Forall_cons_iff in H.
-    destruct H as [H Ht].
-    simpl in *.
-    destruct (lt_dec target nq).
-    + apply Forall_cons.
-      apply den_valid_reset.
-      apply H.
-      apply IHbranches.
-      apply Ht.
-    + apply Forall_cons.
-      apply H.
-      apply IHbranches.
-      apply Ht.
-Qed.
-
-Lemma Execute_suppl_empty_branch: forall (instr: Instruction),
-  Execute_suppl instr [] = [].
-Proof.
-  induction instr.
-  all: try reflexivity.
-  simpl.
-  rewrite IHinstr1.
-  rewrite IHinstr2.
-  reflexivity.
-Qed.
-
-Lemma Execute_suppl_nop: forall (branches: ProgramState),
-  Execute_suppl NopInstr branches = branches.
-Proof.
-  destruct branches.
-  all: reflexivity.
-Qed.
 
 Arguments Execute_rotate_instr _ _ _ _ : simpl never.
 Arguments Execute_cnot_instr _ _ _ : simpl never.
 Arguments Execute_swap_instr _ _ _ : simpl never.
 Arguments Execute_measure_instr _ _ _ : simpl never.
 
-Lemma Execute_suppl_quantum_state_density:
-  forall (instr: Instruction) (branches: ProgramState),
-  Forall qstate_valid branches -> Forall qstate_valid (Execute_suppl instr branches).
+
+Lemma Execute_suppl_valid:
+  forall (instr: Instruction) (ps: ProgramState),
+  ProgramState_valid ps -> ProgramState_valid (Execute_suppl instr ps).
 Proof.
   induction instr.
   all: intros; simpl.
   - exact H.
-  - apply Execute_rotate_instr_quantum_state_density; apply H.
-  - apply Execute_cnot_instr_quantum_state_density; apply H.
-  - apply Execute_swap_instr_quantum_state_density; apply H.
-  - apply Merge_program_state_qstate_valid.
-    apply Execute_measure_instr_quantum_state_density; apply H.
+  - apply Execute_rotate_instr_valid; apply H.
+  - apply Execute_cnot_instr_valid; apply H.
+  - apply Execute_swap_instr_valid; apply H.
+  - apply Execute_measure_instr_valid; apply H.
   - apply IHinstr2; apply IHinstr1; apply H.
-  - apply Forall_concat.
-    apply Forall_map.
-    induction branches.
-    + apply Forall_nil.
-    + apply Forall_cons.
-      * destruct (eqb (B_cstate a n) b).
-        apply IHinstr.
-        all: apply Forall_cons_iff in H.
-        all: destruct H.
-        all: apply Forall_cons.
-        all: try apply H; try apply Forall_nil.
-      * apply IHbranches.
-        apply Forall_cons_iff in H.
-        destruct H.
-        apply H0.
-  - simpl.
-    apply Execute_reset_instr_quantum_state_density.
-    apply H.
+  - apply PProperties.fold_rec_nodep.
+    + unfold ProgramState_valid; intros.
+      apply PFacts.empty_mapsto_iff in H0.
+      contradiction.
+    + intros cstate_fold branch_fold acc Hmaps_fold Hacc_valid.
+      destruct (eqb (CState_read n cstate_fold) b) eqn:Hcond.
+      1: apply IHinstr.
+      all: intros cstate' branch' Hmaps'.
+      all: apply PFacts.add_mapsto_iff in Hmaps'.
+      all: destruct Hmaps' as [[Hcstate_eq Hbranch_eq] | [Hcstate_neq Hmaps_acc]].
+      all: subst.
+      all: apply (H cstate' branch'); try assumption.
+      all: apply PFacts.empty_mapsto_iff in Hmaps_acc.
+      all: contradiction.
+  - apply Execute_reset_instr_valid; apply H.
 Qed.
 
 
-Theorem Execute_quantum_state_density: forall (program: InlinedProgram),
-  Forall qstate_valid (Execute program).
+Theorem Execute_valid: forall (program: InlinedProgram),
+  ProgramState_valid (Execute program).
 Proof.
   intros.
   unfold Execute.
-  apply Execute_suppl_quantum_state_density.
+  apply Execute_suppl_valid.
   unfold ProgramState_init.
-  apply Forall_cons.
-  apply den_valid_init.
-  apply Forall_nil.
+  intros cstate branch Hmaps.
+  apply PFacts.add_mapsto_iff in Hmaps.
+  destruct Hmaps as [[Hcstate_eq Hbranch_eq] | [Hcstate_neq Hmaps_empty]].
+  - rewrite <- Hbranch_eq.
+    unfold Branch_init, Branch_valid; simpl.
+    split.
+    apply den_valid_init.
+    lra.
+  - apply PFacts.empty_mapsto_iff in Hmaps_empty.
+    contradiction.
 Qed.
 
 End PROGRAM.
